Matroid/Graph/Operations/Union.lean
@@ -5,7 +5,7 @@ import Mathlib.Data.Set.Finite.Basic
 variable {α β ι ι' : Type*} {x y z u v w : α} {e f : β} {G G₁ G₂ H H₁ H₂ : Graph α β}
   {F F₁ F₂ : Set β} {X Y : Set α} {s t : Set (Graph α β)}
 
-open Set Function
+open Set Function Partition
 
 namespace Graph
 
@@ -18,7 +18,7 @@ protected def iUnion (G : ι → Graph α β) (hG : Pairwise (Graph.Compatible o
     obtain ⟨i, hab⟩ := by simpa using hab
     obtain ⟨j, hcd⟩ := by simpa using hcd
     have := hab.of_compatible (hG.of_refl i j) hcd.edge_mem
-    apply ((G j).dup_or_dup_of_isLink_of_isLink this hcd).imp <;> rw [Partition.iSup_rel] <;>
+    apply ((G j).dup_or_dup_of_isLink_of_isLink this hcd).imp <;> rw [iSup_rel] <;>
     refine fun _ => Relation.TransGen.single ?_ <;> simp only [iSup_apply, iSup_Prop_eq] <;>
     use j
 
@@ -35,10 +35,11 @@ lemma iUnion_vertexSet (hG : Pairwise (Graph.Compatible on G)) :
   ext x
   simp [mem_iUnion]
 
-lemma iUnion_dup_of_hasSup (hG : Pairwise (Graph.Compatible on G))
-    (hG' : Pairwise (hasSup on G)) :
+@[simp↓]
+lemma iUnion_dup_of_dup_agree (hG : Pairwise (Graph.Compatible on G))
+    (hG' : Pairwise (Dup_agree on G)) :
     (Graph.iUnion G hG).Dup x y ↔ ∃ i, (G i).Dup x y := by
-  simp only [iUnion_dup, Partition.iSup_rel]
+  simp only [iUnion_dup, iSup_rel]
   refine ⟨fun h => ?_, fun h =>  Relation.TransGen.single <| by simpa⟩
   induction h with
   | single hxb => simpa using hxb
@@ -53,6 +54,15 @@ lemma iUnion_dup_of_nodup (hG : Pairwise (Graph.Compatible on G)) [∀ i, Nodup 
     (Graph.iUnion G hG).Dup = Partition.discrete (⋃ i, V(G i)) := by
   simp only [dup_eq_discrete, iUnion_vertexSet]
 
+lemma dup_le_iUnion (hG : Pairwise (Graph.Compatible on G)) (i : ι) :
+    (G i).Dup ≤ (Graph.iUnion G hG).Dup := by
+  rw [← rel_le_iff_le]
+  intro x y hxy
+  simp only [iUnion_dup, iSup_rel]
+  apply Relation.TransGen.single
+  simp only [iSup_apply, iSup_Prop_eq]
+  use i
+
 @[simp]
 lemma iUnion_isLink (hG : Pairwise (Graph.Compatible on G)) :
     (Graph.iUnion G hG).IsLink e x y ↔
@@ -60,31 +70,35 @@ lemma iUnion_isLink (hG : Pairwise (Graph.Compatible on G)) :
   conv_lhs => rw [Graph.iUnion, mk_of_domp_isLink]
   rfl
 
--- @[simp↓]
--- lemma iUnion_isLink_of_hasSup (hG : Pairwise (Graph.Compatible on G))
---     (hG' : Pairwise (hasSup on G)) :
---     (Graph.iUnion G hG).IsLink e x y ↔ ∃ i, (G i).IsLink e x y := by
---   simp only [iUnion_isLink, iUnion_dup, Partition.iSup_rel]
---   refine ⟨fun ⟨a, hxa, b, hlba, hby⟩ => ?_, fun h => ?_⟩
---   ·
---     sorry
---   sorry
+lemma isLink_le_iUnion (hG : Pairwise (Graph.Compatible on G)) (i : ι) :
+    (G i).IsLink e x y ≤ (Graph.iUnion G hG).IsLink e x y := by
+  refine fun hxy ↦ ⟨x, ?_, y, ?_, ?_⟩ <;> simp only [iSup_rel,
+    Relation.transClosure_self_iff, iSup_apply, iSup_Prop_eq, Relation.flip_apply] <;> use i
+  · exact hxy.left_refl
+  · exact symm hxy
+  · exact hxy.right_refl
+
+@[simp↓]
+lemma iUnion_isLink_of_dup_agree (hG : Pairwise (Graph.Compatible on G))
+    (hG' : Pairwise (Dup_agree on G)) :
+    (Graph.iUnion G hG).IsLink e x y ↔ ∃ i, (G i).IsLink e x y := by
+  refine ⟨fun ⟨a, hxa, b, hlba, hby⟩ => ?_, fun ⟨i, hlxy⟩ => isLink_le_iUnion hG i hlxy⟩
+  obtain ⟨i, hlba⟩ := by simpa using hlba
+  rw [dup_of_pairwise_dup_agree_of_mem hG' hlba.left_mem] at hby
+  rw [comm_of (⇑(⨆ i, (G i).Dup)), dup_of_pairwise_dup_agree_of_mem hG' hlba.right_mem] at hxa
+  exact ⟨i, trans' (trans' (symm hxa) hlba.symm) hby⟩
 
 @[simp↓]
 lemma iUnion_isLink_of_nodup (hG : Pairwise (Graph.Compatible on G)) [∀ i, Nodup (G i)] :
-    (Graph.iUnion G hG).IsLink e x y ↔ ∃ i, (G i).IsLink e x y := by
-  simp only [iUnion_isLink, Relation.Domp, Relation.Comp, dup_eq_discrete, iUnion_vertexSet,
-    Partition.rel_discrete_iff, mem_iUnion, Relation.flip_apply, iSup_apply, iSup_Prop_eq,
-    existsAndEq, true_and, isLink_comm]
-  rw [and_comm, and_assoc, and_iff_left_iff_imp, forall_exists_index]
-  exact fun i hl ↦ ⟨⟨i, hl.right_mem⟩, ⟨i, hl.left_mem⟩⟩
+    (Graph.iUnion G hG).IsLink e x y ↔ ∃ i, (G i).IsLink e x y :=
+  iUnion_isLink_of_dup_agree hG pairwise_dup_agree_of_nodup
 
 @[simp]
 lemma iUnion_edgeSet (hG : Pairwise (Graph.Compatible on G)) :
     E(Graph.iUnion G hG) = ⋃ i, E(G i) := by
   rw [Graph.iUnion, mk_of_domp_edgeSet]
   ext e
-  simp +contextual only [Relation.Domp, Relation.Comp, Partition.iSup_rel, Relation.flip_apply,
+  simp +contextual only [Relation.Domp, Relation.Comp, iSup_rel, Relation.flip_apply,
     iSup_apply, iSup_Prop_eq, mem_setOf_eq, mem_iUnion, iff_def, forall_exists_index, and_imp]
   refine ⟨fun a b c hac d i hldc hdb => ⟨i, hldc.edge_mem⟩, fun i hei => ?_⟩
   obtain ⟨x, y, hl⟩ := exists_isLink_of_mem_edgeSet hei
@@ -92,42 +106,28 @@ lemma iUnion_edgeSet (hG : Pairwise (Graph.Compatible on G)) :
   · exact ⟨i, hl.left_refl⟩
   · exact ⟨i, hl.right_refl⟩
 
-lemma dup_le_iUnion (hG : Pairwise (Graph.Compatible on G)) (i : ι) :
-    (G i).Dup ≤ (Graph.iUnion G hG).Dup := by
-  rw [← Partition.rel_le_iff_le]
-  intro x y hxy
-  simp only [iUnion_dup, Partition.iSup_rel]
-  apply Relation.TransGen.single
-  simp only [iSup_apply, iSup_Prop_eq]
-  use i
+protected lemma le_iUnion (hG : Pairwise (Graph.Compatible on G))
+    (hG' : Pairwise (Dup_agree on G)) (i : ι) : G i ≤ Graph.iUnion G hG :=
+  le_of (subset_iSup_of_agree hG' i) (fun _ _ _ ↦ isLink_le_iUnion hG i)
 
-lemma isLink_le_iUnion (hG : Pairwise (Graph.Compatible on G)) (i : ι) :
-    (G i).IsLink e x y ≤ (Graph.iUnion G hG).IsLink e x y := by
-  simp only [iUnion_isLink, iUnion_dup, Partition.iSup_rel, Relation.domp_def', le_Prop_eq]
-  refine fun hxy ↦ ⟨x, Relation.TransGen.single ?_, y, ?_, Relation.TransGen.single ?_⟩ <;>
-    simp only [Relation.flip_apply, iSup_apply, iSup_Prop_eq] <;> use i
-  · exact hxy.left_refl
-  · exact symm hxy
-  · exact hxy.right_refl
-
-protected lemma le_iUnion (hG : Pairwise (Graph.Compatible on G)) (i : ι) [hN : ∀ i, Nodup (G i)] :
-    G i ≤ Graph.iUnion G hG := by
-  refine le_of ?_ (fun _ _ _ ↦ isLink_le_iUnion hG i)
-  simp_rw [dup_eq_discrete, Partition.discrete_subset_discrete_iff, iUnion_vertexSet]
-  exact subset_iUnion_of_subset i fun ⦃a⦄ a ↦ a
+protected lemma le_iUnion_of_nodup (hG : Pairwise (Graph.Compatible on G)) [hN : ∀ i, Nodup (G i)]
+    (i : ι) : G i ≤ Graph.iUnion G hG := Graph.le_iUnion hG pairwise_dup_agree_of_nodup i
 
 @[simp]
-protected lemma iUnion_le_iff (hG : Pairwise (Graph.Compatible on G)) [hN : ∀ i, Nodup (G i)] :
-    Graph.iUnion G hG ≤ H ↔ ∀ i, G i ≤ H := by
-  refine ⟨fun h i ↦ (Graph.le_iUnion hG i).trans h,
-    fun h' ↦ ⟨fun hx ↦ ?_, fun e x y hl ↦ ?_⟩⟩
-  · simp only [dup_eq_discrete, iUnion_vertexSet, Partition.mem_parts, SetLike.mem_coe,
-      Partition.mem_discrete_iff, mem_iUnion, forall_exists_index, and_imp]
-    rintro x i hx rfl
-    refine (h' i).dup_subset ?_
-    simpa
-  obtain ⟨i, hl⟩ := (iUnion_isLink_of_nodup hG).mp hl
+protected lemma iUnion_le_iff (hG : Pairwise (Graph.Compatible on G))
+    (hG' : Pairwise (Dup_agree on G)) : Graph.iUnion G hG ≤ H ↔ ∀ i, G i ≤ H := by
+  refine ⟨fun h i ↦ (Graph.le_iUnion hG hG' i).trans h,
+    fun h' ↦ ⟨fun s hs ↦ ?_, fun e x y hl ↦ ?_⟩⟩
+  · simp only [iUnion_dup, mem_parts, SetLike.mem_coe] at hs
+    obtain ⟨i, hs⟩ := (mem_iSup_iff_of_agree hG').mp hs
+    exact h' i |>.dup_subset hs
+  obtain ⟨i, hl⟩ := (iUnion_isLink_of_dup_agree hG hG').mp hl
   exact hl.of_le (h' i)
+
+@[simp]
+protected lemma iUnion_le_iff_of_nodup (hG : Pairwise (Graph.Compatible on G))
+    [hN : ∀ i, Nodup (G i)] : Graph.iUnion G hG ≤ H ↔ ∀ i, G i ≤ H :=
+  Graph.iUnion_le_iff hG pairwise_dup_agree_of_nodup
 
 @[simp]
 protected lemma iUnion_const [Nonempty ι] (G : Graph α β) :
@@ -148,43 +148,70 @@ lemma iUnion_inc_iff (hG : Pairwise (Graph.Compatible on G)) :
   use i, hlyz.symm
 
 @[simp↓]
-lemma iUnion_inc_iff_of_nodup (hG : Pairwise (Graph.Compatible on G)) [hN : ∀ i, Nodup (G i)] :
+lemma iUnion_inc_iff_of_agree (hG : Pairwise (Graph.Compatible on G))
+    (hG' : Pairwise (Dup_agree on G)) :
     (Graph.iUnion G hG).Inc e x ↔ ∃ i, (G i).Inc e x := by
-  simpa [Inc] using exists_comm
+  simpa [Inc, hG'] using exists_comm
+
+@[simp↓]
+lemma iUnion_inc_iff_of_nodup (hG : Pairwise (Graph.Compatible on G)) [hN : ∀ i, Nodup (G i)] :
+    (Graph.iUnion G hG).Inc e x ↔ ∃ i, (G i).Inc e x := by simp
 
 @[simp]
-lemma iUnion_isLoopAt_iff (hG : Pairwise (Graph.Compatible on G)) [hN : ∀ i, Nodup (G i)] :
+lemma iUnion_isLoopAt_iff_of_agree (hG : Pairwise (Graph.Compatible on G))
+    (hG' : Pairwise (Dup_agree on G)) :
     (Graph.iUnion G hG).IsLoopAt e x ↔ ∃ i, (G i).IsLoopAt e x := by
-  simp [← isLink_self_iff]
+  simp [← isLink_self_iff, hG']
 
 @[simp]
-lemma iUnion_isNonloopAt_iff (hG : Pairwise (Graph.Compatible on G)) [hN : ∀ i, Nodup (G i)] :
+lemma iUnion_isLoopAt_iff_of_nodup (hG : Pairwise (Graph.Compatible on G)) [hN : ∀ i, Nodup (G i)] :
+    (Graph.iUnion G hG).IsLoopAt e x ↔ ∃ i, (G i).IsLoopAt e x := by simp
+
+@[simp]
+lemma iUnion_isNonloopAt_iff (hG : Pairwise (Graph.Compatible on G))
+    (hG' : Pairwise (Dup_agree on G)) :
     (Graph.iUnion G hG).IsNonloopAt e x ↔ ∃ i, (G i).IsNonloopAt e x := by
-  simp only [IsNonloopAt, dup_eq_discrete, iUnion_vertexSet, Partition.rel_discrete_iff, mem_iUnion,
-    not_and, not_exists, ↓iUnion_isLink_of_nodup]
-  refine ⟨fun ⟨z, hnd, i, hil⟩ => ⟨i, z, (hnd · i), hil⟩, fun ⟨i, z, hnd, hil⟩ => ⟨z, ?_, i, hil⟩⟩
-  rintro rfl j
-  exact (hnd rfl hil.left_mem).elim
+  simp only [IsNonloopAt, hG', ↓iUnion_dup_of_dup_agree, not_exists, ↓iUnion_isLink_of_dup_agree]
+  refine ⟨fun ⟨z, hnd, i, hil⟩ => ⟨i, z, hnd i, hil⟩, fun ⟨i, z, hnd, hil⟩ => ⟨z, ?_, i, hil⟩⟩
+  exact fun j hj ↦ hnd <| (hG'.of_refl i j).rel_of_right_of_mem (by simpa using hil.left_mem) hj
+
+@[simp]
+lemma iUnion_isNonloopAt_iff_of_nodup (hG : Pairwise (Graph.Compatible on G))
+    [hN : ∀ i, Nodup (G i)] :
+    (Graph.iUnion G hG).IsNonloopAt e x ↔ ∃ i, (G i).IsNonloopAt e x := by simp
 
 lemma iUnion_map_le_iUnion (hG : Pairwise (Graph.Compatible on G)) (f : ι' → ι)
-    [hN : ∀ i, Nodup (G i)] :
+    (hG' : Pairwise (Dup_agree on G)) :
     (Graph.iUnion (G ∘ f) (pairwise_compatible_comp hG f)) ≤ Graph.iUnion G hG := by
-  rw [Graph.iUnion_le_iff (hN := by simp; infer_instance)]
-  exact fun i ↦ Graph.le_iUnion hG (f i)
-
-lemma iUnion_left_le_iUnion_sum {H : ι' → Graph α β} [∀ i, Nodup (G i)] [∀ i, Nodup (H i)]
-    (hGH : Pairwise (Graph.Compatible on Sum.elim G H))  :
-    Graph.iUnion G hGH.sum_left ≤ Graph.iUnion (Sum.elim G H) hGH := by
   rw [Graph.iUnion_le_iff]
-  exact fun i ↦ le_trans (by simp) (Graph.le_iUnion hGH (Sum.inl i)
-    (hN := by simp; exact ⟨inferInstance, inferInstance⟩))
+  · exact fun i ↦ Graph.le_iUnion hG hG' (f i)
+  apply Pairwise.onFun_of_refl hG'
 
-lemma iUnion_right_le_iUnion_sum {H : ι' → Graph α β} [∀ i, Nodup (G i)] [∀ i, Nodup (H i)]
-    (hGH : Pairwise (Graph.Compatible on Sum.elim G H)) :
-    Graph.iUnion H hGH.sum_right ≤ Graph.iUnion (Sum.elim G H) hGH := by
-  rw [Graph.iUnion_le_iff]
-  exact fun i ↦ le_trans (by simp) (Graph.le_iUnion hGH (Sum.inr i)
-    (hN := by simp; exact ⟨inferInstance, inferInstance⟩))
+lemma iUnion_map_le_iUnion_of_nodup (hG : Pairwise (Graph.Compatible on G)) (f : ι' → ι)
+    [hN : ∀ i, Nodup (G i)] :
+    (Graph.iUnion (G ∘ f) (pairwise_compatible_comp hG f)) ≤ Graph.iUnion G hG :=
+  iUnion_map_le_iUnion hG f pairwise_dup_agree_of_nodup
+
+-- lemma iUnion_left_le_iUnion_sum {H : ι' → Graph α β}
+--     (hGH : Pairwise (Graph.Compatible on Sum.elim G H))
+--     (hG' : Pairwise (Dup_agree on G)) (hH' : Pairwise (Dup_agree on H)) :
+--     Graph.iUnion G hGH.sum_left ≤ Graph.iUnion (Sum.elim G H) hGH := by
+--   rw [Graph.iUnion_le_iff _ hG']
+--   refine fun i ↦ le_trans (by simp) (Graph.le_iUnion hGH ?_ (Sum.inl i))
+--   sorry
+
+-- lemma iUnion_left_le_iUnion_sum_of_nodup {H : ι' → Graph α β} [∀ i, Nodup (G i)]
+-- [∀ i, Nodup (H i)]
+--     (hGH : Pairwise (Graph.Compatible on Sum.elim G H)) :
+--     Graph.iUnion G hGH.sum_left ≤ Graph.iUnion (Sum.elim G H) hGH :=
+--   iUnion_left_le_iUnion_sum hGH pairwise_dup_agree_of_nodup pairwise_dup_agree_of_nodup
+
+-- lemma iUnion_right_le_iUnion_sum {H : ι' → Graph α β} [∀ i, Nodup (G i)] [∀ i, Nodup (H i)]
+--     (hGH : Pairwise (Graph.Compatible on Sum.elim G H)) :
+--     Graph.iUnion H hGH.sum_right ≤ Graph.iUnion (Sum.elim G H) hGH := by
+--   rw [Graph.iUnion_le_iff]
+--   exact fun i ↦ le_trans (by simp) (Graph.le_iUnion hGH (Sum.inr i)
+--     (hN := by simp; exact ⟨inferInstance, inferInstance⟩))
 
 -- @[simp]
 -- lemma induce_iUnion [Nonempty ι] (hG : Pairwise (Graph.Compatible on G)) (X : Set α) :
@@ -202,7 +229,7 @@ lemma Compatible.edgeDelete_iUnion (hG : Pairwise (Graph.Compatible on G))
     (F : Set β) :
     (Graph.iUnion G hG) ＼ F = .iUnion (fun i ↦ (G i) ＼ F) (fun _ _ hij ↦ (hG hij).edgeDelete) := by
   ext <;> simp only [edgeDelete_isLink, iUnion_isLink, Relation.Domp, Relation.Comp, iUnion_dup,
-    Partition.iSup_rel, Relation.flip_apply, iSup_apply, iSup_Prop_eq, edgeDelete_dup,
+    iSup_rel, Relation.flip_apply, iSup_apply, iSup_Prop_eq, edgeDelete_dup,
     exists_and_right]
   tauto
 
@@ -211,30 +238,30 @@ lemma Compatible.edgeRestrict_iUnion (hG : Pairwise (Graph.Compatible on G))
     (F : Set β) : (Graph.iUnion G hG) ↾ F =
     .iUnion (fun i ↦ (G i) ↾ F) (fun _ _ hij ↦ (hG hij).edgeRestrict) := by
   ext <;> simp only [edgeRestrict_isLink, iUnion_isLink, Relation.Domp, Relation.Comp, iUnion_dup,
-    Partition.iSup_rel, Relation.flip_apply, iSup_apply, iSup_Prop_eq, edgeRestrict_dup,
+    iSup_rel, Relation.flip_apply, iSup_apply, iSup_Prop_eq, edgeRestrict_dup,
     exists_and_left]
   tauto
 
-protected lemma iUnion_comp_le {f : ι' → ι} (hG : Pairwise (Compatible on G))
-    [hN : ∀ i, Nodup (G i)] :
-    Graph.iUnion (fun i ↦ G (f i)) (pairwise_compatible_comp hG f) ≤ Graph.iUnion G hG := by
-  rw [Graph.iUnion_le_iff]
-  exact fun i ↦ Graph.le_iUnion hG (f i)
+-- protected lemma iUnion_comp_le {f : ι' → ι} (hG : Pairwise (Compatible on G))
+--     [hN : ∀ i, Nodup (G i)] :
+--     Graph.iUnion (fun i ↦ G (f i)) (pairwise_compatible_comp hG f) ≤ Graph.iUnion G hG := by
+--   rw [Graph.iUnion_le_iff]
+--   exact fun i ↦ Graph.le_iUnion hG (f i)
 
-lemma iUnion_comp_eq_of_surj {f : ι' → ι} (hG : Pairwise (Compatible on G))
-    (hf : Function.Surjective f) [hN : ∀ i, Nodup (G i)] :
-    Graph.iUnion G hG = Graph.iUnion (fun i ↦ G (f i)) (pairwise_compatible_comp hG f) := by
-  refine le_antisymm ?_ (Graph.iUnion_comp_le hG)
-  rw [Graph.iUnion_le_iff]
-  rintro i
-  obtain ⟨i', rfl⟩ := hf i
-  exact Graph.le_iUnion (pairwise_compatible_comp hG f) i' (hN := by simp; infer_instance)
+-- lemma iUnion_comp_eq_of_surj {f : ι' → ι} (hG : Pairwise (Compatible on G))
+--     (hf : Function.Surjective f) [hN : ∀ i, Nodup (G i)] :
+--     Graph.iUnion G hG = Graph.iUnion (fun i ↦ G (f i)) (pairwise_compatible_comp hG f) := by
+--   refine le_antisymm ?_ (Graph.iUnion_comp_le hG)
+--   rw [Graph.iUnion_le_iff]
+--   rintro i
+--   obtain ⟨i', rfl⟩ := hf i
+--   exact Graph.le_iUnion (pairwise_compatible_comp hG f) i' (hN := by simp; infer_instance)
 
-lemma iUnion_range {f : ι' → ι} {G : (Set.range f) → Graph α β}
-    (hG : Pairwise (Graph.Compatible on G)) [hN : ∀ i, Nodup (G i)] :
-    Graph.iUnion G hG = Graph.iUnion (G <| Set.rangeFactorization f ·)
-    (pairwise_compatible_comp hG <| rangeFactorization f) :=
-  iUnion_comp_eq_of_surj hG surjective_onto_range
+-- lemma iUnion_range {f : ι' → ι} {G : (Set.range f) → Graph α β}
+--     (hG : Pairwise (Graph.Compatible on G)) [hN : ∀ i, Nodup (G i)] :
+--     Graph.iUnion G hG = Graph.iUnion (G <| Set.rangeFactorization f ·)
+--     (pairwise_compatible_comp hG <| rangeFactorization f) :=
+--   iUnion_comp_eq_of_surj hG surjective_onto_range
 
 /-! ### Set unions -/
 
@@ -271,9 +298,9 @@ instance (hs : s.Pairwise Compatible) [hN : ∀ (i : s), Nodup i.val] :
   unfold Graph.sUnion
   infer_instance
 
-protected lemma le_sUnion (hs : s.Pairwise Graph.Compatible) (hG : G ∈ s)
-    [hN : ∀ (i : s), Nodup i.val] : G ≤ Graph.sUnion s hs := by
-  exact Graph.le_iUnion (ι := s) _ ⟨G, hG⟩ (hN := hN)
+-- protected lemma le_sUnion (hs : s.Pairwise Graph.Compatible) (hG : G ∈ s)
+--     [hN : ∀ (i : s), Nodup i.val] : G ≤ Graph.sUnion s hs := by
+--   exact Graph.le_iUnion (ι := s) _ ⟨G, hG⟩ (hN := hN)
 
 @[simp]
 protected lemma sUnion_le_iff (hs : s.Pairwise Graph.Compatible) [hN : ∀ (i : s), Nodup i.val]:
@@ -291,10 +318,10 @@ lemma sUnion_inc_iff_of_nodup (hs : s.Pairwise Graph.Compatible) [hN : ∀ (i : 
   rw [Graph.sUnion, iUnion_inc_iff_of_nodup]
   simp
 
-@[simp]
-lemma sUnion_isLoopAt_iff (hs : s.Pairwise Graph.Compatible) [hN : ∀ (i : s), Nodup i.val]:
-    (Graph.sUnion s hs).IsLoopAt e x ↔ ∃ G ∈ s, G.IsLoopAt e x := by
-  simp [Graph.sUnion, iUnion_isLoopAt_iff]
+-- @[simp]
+-- lemma sUnion_isLoopAt_iff (hs : s.Pairwise Graph.Compatible) [hN : ∀ (i : s), Nodup i.val]:
+--     (Graph.sUnion s hs).IsLoopAt e x ↔ ∃ G ∈ s, G.IsLoopAt e x := by
+--   simp [Graph.sUnion, iUnion_isLoopAt_iff]
 
 @[simp]
 lemma sUnion_isNonloopAt_iff (hs : s.Pairwise Graph.Compatible) [hN : ∀ (i : s), Nodup i.val]:
@@ -309,22 +336,22 @@ protected lemma sUnion_singleton (G : Graph α β) : Graph.sUnion {G} (by simp) 
     exact x.prop
   exact instNonemptyOfInhabited
 
-protected lemma sUnion_image {s : Set ι} {f : ι → Graph α β}
-    (hs : s.Pairwise (Graph.Compatible on f)) [hN : ∀ i, Nodup (f i)] :
-    Graph.sUnion (f '' s) hs.image = .iUnion (f · : s → _) (Pairwise.restrict.mpr hs) := by
-  rw [Graph.sUnion]
-  let f' : s → ↑(f '' s) := fun i ↦ ⟨f i, ⟨i, i.2, rfl⟩⟩
-  convert Graph.iUnion_comp_eq_of_surj (f := f') _ (fun ⟨_, i, hGs, rfl⟩ ↦ ⟨⟨i, hGs⟩, rfl⟩)
-  rintro ⟨_, i, _, rfl⟩
-  exact hN i
+-- protected lemma sUnion_image {s : Set ι} {f : ι → Graph α β}
+--     (hs : s.Pairwise (Graph.Compatible on f)) [hN : ∀ i, Nodup (f i)] :
+--     Graph.sUnion (f '' s) hs.image = .iUnion (f · : s → _) (Pairwise.restrict.mpr hs) := by
+--   rw [Graph.sUnion]
+--   let f' : s → ↑(f '' s) := fun i ↦ ⟨f i, ⟨i, i.2, rfl⟩⟩
+--   convert Graph.iUnion_comp_eq_of_surj (f := f') _ (fun ⟨_, i, hGs, rfl⟩ ↦ ⟨⟨i, hGs⟩, rfl⟩)
+--   rintro ⟨_, i, _, rfl⟩
+--   exact hN i
 
-protected lemma sUnion_range {f : ι → Graph α β} (h : Pairwise (Graph.Compatible on f))
-    [hN : ∀ i, Nodup (f i)] :
-    Graph.sUnion (Set.range f) h.range_pairwise = .iUnion f h := by
-  unfold Graph.sUnion
-  convert Graph.iUnion_comp_eq_of_surj (f := Set.rangeFactorization f) _ surjective_onto_range
-  rintro ⟨_, i, _, rfl⟩
-  exact hN i
+-- protected lemma sUnion_range {f : ι → Graph α β} (h : Pairwise (Graph.Compatible on f))
+--     [hN : ∀ i, Nodup (f i)] :
+--     Graph.sUnion (Set.range f) h.range_pairwise = .iUnion f h := by
+--   unfold Graph.sUnion
+--   convert Graph.iUnion_comp_eq_of_surj (f := Set.rangeFactorization f) _ surjective_onto_range
+--   rintro ⟨_, i, _, rfl⟩
+--   exact hN i
 
 /-! ### Unions of pairs -/
 
@@ -396,9 +423,9 @@ lemma union_inc_iff_of_nodup [Nodup G] [Nodup H] :
   rw [union_eq_sUnion, sUnion_inc_iff_of_nodup]
   simp
 
-lemma union_isLoopAt_iff [Nodup G] [Nodup H] :
-    (G ∪ H).IsLoopAt e x ↔ G.IsLoopAt e x ∨ (H.IsLoopAt e x ∧ e ∉ E(G)) := by
-  simp [union_eq_sUnion]
+-- lemma union_isLoopAt_iff [Nodup G] [Nodup H] :
+--     (G ∪ H).IsLoopAt e x ↔ G.IsLoopAt e x ∨ (H.IsLoopAt e x ∧ e ∉ E(G)) := by
+--   simp [union_eq_sUnion]
 
 lemma union_isNonloopAt_iff [Nodup G] [Nodup H] :
     (G ∪ H).IsNonloopAt e x ↔ G.IsNonloopAt e x ∨ (H.IsNonloopAt e x ∧ e ∉ E(G)) := by
@@ -422,12 +449,12 @@ lemma union_le_iff {H₁ H₂ : Graph α β} [h₁ : Nodup H₁] [h₂ : Nodup H
     H₁ ∪ H₂ ≤ G ↔ H₁ ≤ G ∧ H₂ ＼ E(H₁) ≤ G := by
   simp [union_eq_sUnion]
 
-lemma union_mono_right [Nodup G] [Nodup H₂] (h : H₁ ≤ H₂) : G ∪ H₁ ≤ G ∪ H₂ := by
-  let _ := Nodup.of_le h
-  simp only [union_eq_sUnion, Graph.sUnion_le_iff, mem_insert_iff, mem_singleton_iff,
-    forall_eq_or_imp, forall_eq]
-  exact ⟨Graph.le_sUnion _ (by simp), le_trans (edgeDelete_mono_left h) <|
-    Graph.le_sUnion _ (by simp : H₂ ＼ E(G) ∈ _)⟩
+-- lemma union_mono_right [Nodup G] [Nodup H₂] (h : H₁ ≤ H₂) : G ∪ H₁ ≤ G ∪ H₂ := by
+--   let _ := Nodup.of_le h
+--   simp only [union_eq_sUnion, Graph.sUnion_le_iff, mem_insert_iff, mem_singleton_iff,
+--     forall_eq_or_imp, forall_eq]
+--   exact ⟨Graph.le_sUnion _ (by simp), le_trans (edgeDelete_mono_left h) <|
+--     Graph.le_sUnion _ (by simp : H₂ ＼ E(G) ∈ _)⟩
 
 @[simp]
 protected lemma union_self (G : Graph α β) [Nodup G] : G ∪ G = G :=
@@ -500,13 +527,13 @@ lemma Compatible.union_inc_iff_of_nodup [Nodup G] [Nodup H] (h : G.Compatible H)
     exact (·.of_compatible h.symm heG)
   simp [heG]
 
-lemma Compatible.union_isLoopAt_iff [Nodup G] [Nodup H] (h : G.Compatible H) :
-    (G ∪ H).IsLoopAt e x ↔ G.IsLoopAt e x ∨ H.IsLoopAt e x := by
-  rw [Graph.union_isLoopAt_iff]
-  by_cases heG : e ∈ E(G)
-  · simp only [heG, not_true_eq_false, and_false, or_false, iff_self_or]
-    exact (·.of_compatible h.symm heG)
-  simp [heG]
+-- lemma Compatible.union_isLoopAt_iff [Nodup G] [Nodup H] (h : G.Compatible H) :
+--     (G ∪ H).IsLoopAt e x ↔ G.IsLoopAt e x ∨ H.IsLoopAt e x := by
+--   rw [Graph.union_isLoopAt_iff]
+--   by_cases heG : e ∈ E(G)
+--   · simp only [heG, not_true_eq_false, and_false, or_false, iff_self_or]
+--     exact (·.of_compatible h.symm heG)
+--   simp [heG]
 
 -- lemma Compatible.union_isNonloopAt_iff [Nodup G] [Nodup H] (h : G.Compatible H) :
 --     (G ∪ H).IsNonloopAt e x ↔ G.IsNonloopAt e x ∨ H.IsNonloopAt e x := by
@@ -556,15 +583,15 @@ lemma union_eq_self_of_le_left [Nodup G] [Nodup H] (hle : G ≤ H) : G ∪ H = H
 lemma union_eq_self_of_le_right [Nodup G] [Nodup H] (hle : G ≤ H) : H ∪ G = H :=
   (Graph.union_le rfl.le hle).antisymm <| Graph.left_le_union ..
 
-lemma Compatible.union_mono_left [Nodup G] [Nodup H₂] (h : H₂.Compatible G)
-    (hle : H₁ ≤ H₂) : H₁ ∪ G ≤ H₂ ∪ G := by
-  rw [h.union_comm, (h.mono_left hle).union_comm]
-  exact union_mono_right hle
+-- lemma Compatible.union_mono_left [Nodup G] [Nodup H₂] (h : H₂.Compatible G)
+--     (hle : H₁ ≤ H₂) : H₁ ∪ G ≤ H₂ ∪ G := by
+--   rw [h.union_comm, (h.mono_left hle).union_comm]
+--   exact union_mono_right hle
 
-lemma Compatible.union_mono [Nodup G₂] [Nodup H₂] (hleG : G₁ ≤ G₂)
-    (hleH : H₁ ≤ H₂) (h : G₂.Compatible H₁) : G₁ ∪ H₁ ≤ G₂ ∪ H₂ :=
-  let _ := Nodup.of_le hleH
-  le_trans (h.union_mono_left hleG) (union_mono_right hleH)
+-- lemma Compatible.union_mono [Nodup G₂] [Nodup H₂] (hleG : G₁ ≤ G₂)
+--     (hleH : H₁ ≤ H₂) (h : G₂.Compatible H₁) : G₁ ∪ H₁ ≤ G₂ ∪ H₂ :=
+--   let _ := Nodup.of_le hleH
+--   le_trans (h.union_mono_left hleG) (union_mono_right hleH)
 
 -- Remove Nodup assumption
 lemma edgeRestrict_union_edgeDelete (G : Graph α β) [Nodup G] (F : Set β) :
