Matroid/ForMathlib/Partition/Lattice.lean
@@ -69,6 +69,29 @@ lemma sup_rel (P Q : Partition (Set α)) : ⇑(P ⊔ Q) = TransClosure (⇑P ⊔
   change ⇑(ofRel _) = _
   rw [rel_ofRel_eq]
 
+@[simp↓]
+lemma Agree.sup_rel (hPQ : P.Agree Q) : ⇑(P ⊔ Q) = ⇑P ⊔ ⇑Q := by
+  ext x y
+  rw [Partition.sup_rel]
+  refine ⟨fun h => ?_, TransGen.single⟩
+  induction h with
+  | single hxy => exact hxy
+  | tail _ hxy IH => exact hPQ.sup_rel_trans IH hxy
+
+lemma Agree.sup_rel_left_of_mem (hPQ : P.Agree Q) (hx : x ∈ P.supp) : ⇑(P ⊔ Q) x y ↔ ⇑P x y := by
+  rw [hPQ.sup_rel]
+  refine ⟨fun h => ?_, fun h => by aesop⟩
+  obtain (hP | hQ) := h
+  · exact hP
+  exact hPQ.rel_of_right_of_mem hx hQ
+
+lemma Agree.sup_rel_right_of_mem (hPQ : P.Agree Q) (hx : x ∈ Q.supp) : ⇑(P ⊔ Q) x y ↔ ⇑Q x y := by
+  rw [hPQ.sup_rel]
+  refine ⟨fun h => ?_, fun h => by aesop⟩
+  obtain (hP | hQ) := h
+  · exact hPQ.rel_of_left_of_mem hx hP
+  exact hQ
+
 @[simp]
 lemma inf_rel (P Q : Partition (Set α)) : ⇑(P ⊓ Q) = ⇑P ⊓ ⇑Q := by
   change ⇑(ofRel _) = _
@@ -78,6 +101,28 @@ lemma inf_rel (P Q : Partition (Set α)) : ⇑(P ⊓ Q) = ⇑P ⊓ ⇑Q := by
 lemma sSup_rel (S : Set (Partition (Set α))) : ⇑(sSup S) = TransClosure (sSup <| (⇑) '' S) := by
   change ⇑(ofRel _) = _
   rw [rel_ofRel_eq]
+
+@[simp↓]
+lemma sSup_rel_of_agree {S : Set (Partition (Set α))} (hS : S.Pairwise Agree) :
+    ⇑(sSup S) = (sSup <| (⇑) '' S) := by
+  ext x y
+  rw [Partition.sSup_rel]
+  refine ⟨fun h => ?_, TransGen.single⟩
+  induction h with
+  | single hxy => exact hxy
+  | tail _ hxy IH =>
+    simp only [sSup_apply, iSup_apply, iSup_Prop_eq, Subtype.exists, mem_image, exists_prop,
+      exists_exists_and_eq_and] at hxy IH ⊢
+    obtain ⟨Q, hQS, hQ⟩ := hxy
+    obtain ⟨P, hPS, hP⟩ := IH
+    exact ⟨P, hPS, (hS.of_refl hPS hQS).trans_left hP hQ⟩
+
+lemma sSup_rel_of_agree_of_mem {S : Set (Partition (Set α))} (hS : S.Pairwise Agree) (hP : P ∈ S)
+    (hx : x ∈ P.supp) : ⇑(sSup S) x y ↔ ⇑P x y := by
+  rw [sSup_rel_of_agree hS]
+  simp only [sSup_apply, iSup_apply, iSup_Prop_eq, Subtype.exists, mem_image, exists_prop,
+    exists_exists_and_eq_and]
+  exact ⟨fun ⟨Q, hQ, hQx⟩ => (hS.of_refl hP hQ).rel_of_right_of_mem hx hQx, fun h => ⟨P, hP, h⟩⟩
 
 @[simp]
 lemma sInf_rel (S : Set (Partition (Set α))) : ⇑(sInf S) = sInf ((⇑) '' S) := by
@@ -90,6 +135,19 @@ lemma iSup_rel {ι : Type*} (G : ι → Partition (Set α)) :
   change ⇑(ofRel _) = _
   rw [rel_ofRel_eq, iSup, ← range_comp]
   rfl
+
+@[simp↓]
+lemma iSup_rel_of_agree {ι : Type*} {S : ι → Partition (Set α)} (hS : Pairwise (Agree on S)) :
+    ⇑(⨆ i, S i) = (⨆ i, ⇑(S i)) := by
+  convert sSup_rel_of_agree hS.range_pairwise
+  rw [← range_comp]
+  rfl
+
+lemma iSup_rel_of_agree_of_mem {ι : Type*} {S : ι → Partition (Set α)} (hS : Pairwise (Agree on S))
+    (i : ι) (hx : x ∈ (S i).supp) : ⇑(⨆ i, S i) x y ↔ ⇑(S i) x y := by
+  rw [iSup_rel_of_agree hS]
+  simp only [iSup_apply, iSup_Prop_eq]
+  exact ⟨fun ⟨j, hj⟩ => (hS.of_refl i j).rel_of_right_of_mem hx hj, fun h => ⟨i, h⟩⟩
 
 @[simp]
 lemma iInf_rel {ι : Type*} (G : ι → Partition (Set α)) :
@@ -144,6 +202,191 @@ lemma inf_supp (P Q : Partition (Set α)) : (P ⊓ Q).supp = P.supp ∩ Q.supp :
   rw [← sInf_pair, sInf_supp]
   simp
 
+@[simp]
+lemma Agree.subset_sup_left (hPQ : P.Agree Q) : P ⊆ P ⊔ Q := by
+  rw [subset_iff_rel, hPQ.sup_rel]
+  simp only [Pi.sup_apply, sup_Prop_eq, iff_self_or]
+  exact fun _ _ ↦ rel_of_right_of_mem hPQ
+
+@[simp]
+lemma Agree.subset_sup_right (hPQ : P.Agree Q) : Q ⊆ P ⊔ Q := by
+  rw [sup_comm]
+  exact hPQ.symm.subset_sup_left
+
+@[simp]
+lemma subset_sSup_of_agree {S : Set (Partition (Set α))} (hS : S.Pairwise Agree) (hP : P ∈ S) :
+    P ⊆ sSup S := by
+  rw [subset_iff_rel, sSup_rel]
+  refine fun x y hxP ↦ ⟨fun hxy => TransGen.single ?_, fun hxy => ?_⟩
+  · simp only [sSup_apply, iSup_apply, iSup_Prop_eq, Subtype.exists, mem_image, exists_prop,
+    exists_exists_and_eq_and]
+    use P
+  induction hxy with
+  | single hxy =>
+    obtain ⟨Q, hQS, hQ⟩ := by simpa using hxy
+    exact (hS.of_refl hP hQS).trans_left (rel_self_of_mem_supp hxP) hQ
+  | tail _ hxy IH =>
+    obtain ⟨Q, hQS, hQ⟩ := by simpa using hxy
+    exact (hS.of_refl hP hQS).trans_left IH hQ
+
+@[simp]
+lemma subset_iSup_of_agree {ι : Type*} {P : ι → Partition (Set α)} (hP : Pairwise (Agree on P))
+    (i : ι) : P i ⊆ ⨆ i, P i :=
+  subset_sSup_of_agree hP.range_pairwise <| mem_range_self i
+
+@[simp]
+lemma Agree.inf_subset_left (hPQ : P.Agree Q) : P ⊓ Q ⊆ P := by
+  rw [agree_iff_rel] at hPQ
+  rw [subset_iff_rel, inf_rel]
+  refine fun x y hxP ↦ ⟨(·.1), fun hxy => ⟨hxy, ?_⟩⟩
+  rw [inf_supp] at hxP
+  rwa [← hPQ x _ hxP.1 hxP.2]
+
+@[simp]
+lemma Agree.inf_subset_right (hPQ : P.Agree Q) : P ⊓ Q ⊆ Q := by
+  rw [inf_comm]
+  exact hPQ.symm.inf_subset_left
+
+@[simp]
+lemma sInf_subset_of_agree {S : Set (Partition (Set α))} (hS : S.Pairwise Agree) (hP : P ∈ S) :
+    sInf S ⊆ P := by
+  rw [subset_iff_rel]
+  simp only [sInf_supp, mem_iInter, sInf_rel, sInf_apply, iInf_apply, iInf_Prop_eq, Subtype.forall,
+    mem_image, forall_exists_index, and_imp, forall_apply_eq_imp_iff₂]
+  exact fun x y hxP ↦ ⟨fun hxy => hxy P hP,
+    fun hxy Q hQS => (hS.of_refl hQS hP).trans_left (rel_self_of_mem_supp (hxP Q hQS)) hxy⟩
+
+@[simp]
+lemma iInf_subset_of_agree {ι : Type*} {P : ι → Partition (Set α)} (hP : Pairwise (Agree on P))
+    (i : ι) : ⨅ i, P i ⊆ P i :=
+  sInf_subset_of_agree hP.range_pairwise <| mem_range_self i
+
+@[simp]
+lemma Agree.sup_parts (hPQ : P.Agree Q) : (P ⊔ Q) = P.parts ∪ Q.parts := by
+  refine subset_antisymm ?_ <| union_subset hPQ.subset_sup_left hPQ.subset_sup_right
+  rintro s ⟨x, hx, rfl⟩
+  simp only [transClosure_codomain, mem_codomain_iff, Pi.sup_apply, sup_Prop_eq, mem_union,
+    mem_parts, SetLike.mem_coe] at hx ⊢
+  obtain ⟨y, hPyx | hQyx⟩ := hx
+  · left
+    convert partOf_mem hPyx.right_mem using 1
+    ext z
+    rw [mem_fiber_iff, mem_partOf_iff, ← Partition.sup_rel, rel_comm, rel_comm (x := z)]
+    exact hPQ.sup_rel_left_of_mem hPyx.right_mem
+  right
+  convert partOf_mem hQyx.right_mem using 1
+  ext z
+  rw [mem_fiber_iff, mem_partOf_iff, ← Partition.sup_rel, rel_comm, rel_comm (x := z)]
+  exact hPQ.sup_rel_right_of_mem hQyx.right_mem
+
+@[simp]
+lemma Agree.mem_sup_iff (hPQ : P.Agree Q) : s ∈ P ⊔ Q ↔ s ∈ P ∨ s ∈ Q := by
+  change s ∈ (P ⊔ Q).parts ↔ _
+  rw [mem_parts, hPQ.sup_parts]
+  simp
+
+@[simp]
+lemma sSup_parts_of_agree {S : Set (Partition (Set α))} (hS : S.Pairwise Agree) :
+    sSup S = ⋃ P ∈ S, P.parts := by
+  refine subset_antisymm ?_ ?_; swap
+  · simp only [iUnion_subset_iff]
+    exact fun _ => subset_sSup_of_agree hS
+  rintro s ⟨x, hx, rfl⟩
+  simp only [transClosure_codomain, mem_codomain_iff, sSup_apply, iSup_apply, iSup_Prop_eq,
+    Subtype.exists, mem_image, exists_prop, exists_exists_and_eq_and, mem_iUnion, mem_parts,
+    SetLike.mem_coe] at hx ⊢
+  obtain ⟨y, P, hPS, hPyx⟩ := hx
+  use P, hPS
+  convert partOf_mem hPyx.right_mem using 1
+  ext z
+  rw [mem_fiber_iff, mem_partOf_iff, ← Partition.sSup_rel, rel_comm, rel_comm (x := z)]
+  exact sSup_rel_of_agree_of_mem hS hPS hPyx.right_mem
+
+@[simp]
+lemma mem_sSup_iff_of_agree {S : Set (Partition (Set α))} (hS : S.Pairwise Agree) :
+    s ∈ sSup S ↔ ∃ P ∈ S, s ∈ P := by
+  change s ∈ (sSup S).parts ↔ ∃ P ∈ S, s ∈ P
+  rw [mem_parts, sSup_parts_of_agree hS]
+  simp
+
+@[simp]
+lemma iSup_parts_of_agree {ι : Type*} {S : ι → Partition (Set α)} (hS : Pairwise (Agree on S)) :
+    ⨆ i, S i = ⋃ i, (S i).parts := by
+  rw [iSup, sSup_parts_of_agree hS.range_pairwise]
+  simp
+
+@[simp]
+lemma mem_iSup_iff_of_agree {ι : Type*} {S : ι → Partition (Set α)} (hS : Pairwise (Agree on S)) :
+    s ∈ ⨆ i, S i ↔ ∃ i, s ∈ (S i) := by
+  change s ∈ (⨆ i, S i).parts ↔ ∃ i, s ∈ (S i)
+  rw [mem_parts, iSup_parts_of_agree hS]
+  simp
+
+@[simp]
+lemma Agree.inf_parts (hPQ : P.Agree Q) : P ⊓ Q = P.parts ∩ Q.parts := by
+  refine subset_antisymm (subset_inter hPQ.inf_subset_left hPQ.inf_subset_right) ?_
+  rintro s ⟨hsP, hsQ⟩
+  simp only [mem_parts, SetLike.mem_coe] at hsP hsQ ⊢
+  obtain ⟨x, hxs, rfl⟩ := exists_partOf_iff_mem.mp hsP
+  obtain ⟨_, H⟩ := partOf_mem_iff_rel_iff.mp hsQ
+  simp_rw [rel_comm (x := x)] at H
+  use x, ?_
+  · ext y
+    simp [H]
+  simp only [mem_codomain_iff, Pi.inf_apply, ← H, min_self]
+  exact ⟨x, rel_self_of_mem_supp hxs⟩
+
+@[simp]
+lemma Agree.mem_inf_iff (hPQ : P.Agree Q) : s ∈ P ⊓ Q ↔ s ∈ P ∧ s ∈ Q := by
+  change s ∈ (P ⊓ Q).parts ↔ _
+  rw [mem_parts, hPQ.inf_parts]
+  simp
+
+@[simp]
+lemma sInf_parts_of_agree {S : Set (Partition (Set α))} (hS : S.Pairwise Agree) (hS' : S.Nonempty) :
+    sInf S = ⋂ P ∈ S, P.parts := by
+  refine subset_antisymm ?_ ?_
+  · simp only [subset_iInter_iff]
+    exact fun _ => sInf_subset_of_agree hS
+  rintro s hs
+  rw [SetLike.mem_coe, exists_partOf_iff_mem]
+  simp only [mem_iInter, mem_parts, SetLike.mem_coe, sInf, ofRel_supp, mem_domain_iff, iInf_apply,
+    iInf_Prop_eq, Subtype.forall, mem_image, forall_exists_index, and_imp,
+    forall_apply_eq_imp_iff₂] at hs ⊢
+  have hs' := hs hS'.some hS'.some_mem
+  obtain ⟨x, hx⟩ := nonempty_of_mem hs'
+  use x, ?_
+  · ext y
+    simp only [mem_partOf_iff, rel_ofRel_eq, iInf_apply, iInf_Prop_eq, Subtype.forall, mem_image,
+      forall_exists_index, and_imp, forall_apply_eq_imp_iff₂]
+    refine ⟨fun h => ?_, fun h => ?_⟩
+    · obtain ⟨t, ht, hyt, hxt⟩ := h hS'.some hS'.some_mem
+      obtain rfl := eq_of_mem_of_mem ht hs' hxt hx
+      exact hyt
+    rintro P hPS
+    use s, hs P hPS
+  use x
+  exact fun P hPS => rel_of_mem_of_mem (hs P hPS) hx hx
+
+@[simp]
+lemma mem_sInf_iff_of_agree {S : Set (Partition (Set α))} (hS : S.Pairwise Agree)
+    (hS' : S.Nonempty) : s ∈ sInf S ↔ ∀ P ∈ S, s ∈ P := by
+  change s ∈ (sInf S).parts ↔ ∀ P ∈ S, s ∈ P
+  rw [mem_parts, sInf_parts_of_agree hS hS']
+  simp
+
+@[simp]
+lemma iInf_parts_of_agree {ι : Type*} [Nonempty ι] {S : ι → Partition (Set α)}
+    (hS : Pairwise (Agree on S)) : ⨅ i, S i = ⋂ i, (S i).parts := by
+  rw [iInf, sInf_parts_of_agree hS.range_pairwise (range_nonempty S)]
+  simp
+
+@[simp]
+lemma mem_iInf_iff_of_agree {ι : Type*} [Nonempty ι] {S : ι → Partition (Set α)}
+    (hS : Pairwise (Agree on S)) : s ∈ ⨅ i, S i ↔ ∀ i, s ∈ (S i) := by
+  change s ∈ (⨅ i, S i).parts ↔ ∀ i, s ∈ (S i)
+  rw [mem_parts, iInf_parts_of_agree hS]
+  simp
 
 @[simp]
 lemma sSup_atomic {S : Set (Partition (Set α))} (hS : ∀ P ∈ S, P.Atomic) :
